ems/SimGlobalExplicit2AltExp.v
@@ -1,0 +1,34 @@
+Require Import Coqlib.
+Require Import ITreelib.
+Require Import Any.
+Require Import STS.
+Require Import Behavior.
+Require Import ModSem.
+Require Import Skeleton.
+Require Import Coq.Relations.Relation_Definitions.
+Require Import Relation_Operators.
+Require Import RelationPairs.
+From Ordinal Require Import Ordinal Arithmetic.
+From Ordinal Require Import ClassicalOrdinal.
+
+Require Import WFLib.
+Require Import SimGlobalExplicit SimGlobalAlts.
+
+Set Implicit Arguments.
+
+Section PROOF.
+
+  Theorem simg_exp_implies_simg_alt_exp
+          R0 R1 (RR: R0 -> R1 -> Prop)
+          (itr_src: itree eventE R0)
+          (itr_tgt: itree eventE R1)
+          (wf_exp: WF)
+          (e_src e_tgt: wf_exp.(T))
+          (SIM: simg_exp wf_exp RR e_src e_tgt (itr_src) (itr_tgt))
+    :
+    exists wfo f_tgt,
+      simg_alt_exp wfo RR f_tgt itr_src itr_tgt.
+  Proof.
+
+
+End PROOF.
